examples/relational/new/ifc.fst
@@ -30,10 +30,15 @@ let join l1 l2 =
   | Low, Low -> Low
   | _, _     -> High
 
-type label_fun = ref int -> Tot label
+(*
+ * function from the addr_of refs to label
+ *)
+type label_fun = nat -> GTot label
+
+let label_of (env:label_fun) (r:id) :GTot label = env (addr_of r)
 
 type low_equiv (env:label_fun) (h1:rel heap) = 
-  forall (x:ref int). env x = Low ==> sel (R?.l h1) x = sel (R?.r h1) x
+  forall (x:ref int). label_of env x = Low ==> sel (R?.l h1) x = sel (R?.r h1) x
 
 
 (**************************** Typing Judgements ****************************)
@@ -71,7 +76,7 @@ type ni_com' (env:label_fun) (c:com) (l:label) (h0: rel (option heap)) =
     (Some? (R?.r h0) ==>
      (let hr = Some?.v (R?.r h0) in
       let o_r = interpret_com hr c in
-        (forall r. (env r < l /\ Some? o_r)
+        (forall r. (label_of env r < l /\ Some? o_r)
           ==> sel hr r = sel (Some?.v o_r) r)))
 
 type ni_com (env:label_fun) (c:com) (l:label) = 
@@ -107,7 +112,7 @@ let sub_exp _ _ _ _ = ()
 
 val avar_exp : env:label_fun -> r:id -> 
   Lemma (requires True)
-        (ensures  (ni_exp env (AVar r) (env r))) 
+        (ensures  (ni_exp env (AVar r) (label_of env r))) 
 let avar_exp _ _ = ()
 
 
@@ -161,8 +166,8 @@ let sub_com _ _ _ _ = ()
       (first one to prevent explicit, second to prevent implicit flows)
 *)
 val assign_com : env:label_fun -> e:exp -> r:id -> 
-  Lemma (requires (ni_exp env e (env r)))
-        (ensures  (ni_com env (Assign r e) (env r)))
+  Lemma (requires (ni_exp env e (label_of env r)))
+        (ensures  (ni_com env (Assign r e) (label_of env r)))
 let assign_com _ _ _ = ()
 
 (* Sequencing rule for commands
@@ -234,7 +239,7 @@ val while_com' : env:label_fun -> e:exp -> c:com -> v:variant -> l:label -> h:re
         (ensures  (ni_com' env (While e c v) l h)) 
         (decreases (decr_while (R?.l h) v + decr_while (R?.r h) v))
 let rec while_com' env e c v l h = 
-  // Interpret the body
+  (* Interpret the body *)
   match h with
   | R None None -> ()
   | R (Some h_l) None ->
@@ -264,11 +269,11 @@ let rec while_com' env e c v l h =
     let o_l = interpret_com h_l c in 
     let o_r = interpret_com h_r c in 
 
-    // Case analysis on termination of bodies
+    (* Case analysis on termination of bodies *)
     match o_l, o_r with
     | Some hl , Some hr  -> 
       begin
-        // case analysis on decreasing of variant
+        (* case analysis on decreasing of variant *)
         match (interpret_exp h_l v > interpret_exp hl v) && interpret_exp hl v >= 0 , 
           (interpret_exp h_r v > interpret_exp hr v) && interpret_exp hr v >= 0 with
         | true , true  -> while_com' env e c v l (R o_l o_r)
